\section{Equivalent Notions of Advantage}\label{app:calculus}
In this appendix, we prove the following claim:
\begin{claim}
    It holds that
    \begin{equation*}
        2\cdot\tilde{\mathbf{Adv}}_\adv^{\M{G}^0,\M{G}^1}(\lambda)=\mathbf{Adv}_\adv^{\M{G}^0,\M{G}^1}(\lambda),
    \end{equation*}
    where
    \[\mathbf{Adv}_\adv^{\M{G}^0,\M{G}^1}(\lambda):=\abs{\prob{1 = \adv \circ \M{G}^0} - \prob{1 = \adv \circ \M{G}^1}}\]
    and
    \[\tilde{\mathbf{Adv}}_\adv^{\M{G}^0,\M{G}^1}(\lambda):=\abs{\probsub{b\sample\bin}{b = \adv \circ \M{G}^b} - \frac{1}{2}}.\]
\end{claim}
\begin{proof}
    \begin{align*}
        \mathbf{Adv}_\adv^{\M{G}^0,\M{G}^1}(\lambda)                                                                                      \\
        = & \abs{\prob{1 = \adv \circ \M{G}^0} - \prob{1 = \adv \circ \M{G}^1}}                                                           \\
        = & \abs{\prob{1 = \adv \circ \M{G}^1}-\prob{1 = \adv \circ \M{G}^0}}                                                             \\
        = & \abs{-\prob{1 = \adv \circ \M{G}^0} + \prob{1 = \adv \circ \M{G}^1}}                                                          \\
        = & \abs{(1-\prob{1 = \adv \circ \M{G}^0}) + \prob{1 = \adv \circ \M{G}^1} - 1}                                                   \\
        = & 2\cdot\abs{\frac{1}{2}\cdot (1-\prob{1 = \adv \circ \M{G}^0}) + \frac{1}{2}\cdot \prob{1 = \adv \circ \M{G}^1} - \frac{1}{2}} \\
        = & 2\cdot\abs{\frac{1}{2}\cdot \prob{0 = \adv \circ \M{G}^0} + \frac{1}{2}\cdot \prob{1 = \adv \circ \M{G}^1} - \frac{1}{2}}     \\
        = & 2\cdot\abs{\probsub{b\sample\bin}{b = \adv \circ \M{G}^b} - \frac{1}{2}}                                                      \\
        = & 2\cdot\tilde{\mathbf{Adv}}_\adv^{\M{G}^0,\M{G}^1}(\lambda)                                                                    \\
    \end{align*}
\end{proof}
